pulse/lib/pulse/lib/Pulse.Lib.GhostPCMReference.fst
@@ -12,20 +12,7 @@ let pts_to
 : storable
 = ghost_pcm_pts_to #_ #(PR.raise p) r (U.raise_val v)
 
-```pulse
-ghost
-fn alloc (#a:Type u#0) (#p:pcm a) (x:erased a { p.refine x })
-requires emp
-returns r:gref p
-ensures pts_to r x
-{
-  let r = ghost_alloc #_ #(PR.raise p) (U.raise_val x);
-  rewrite ghost_pcm_pts_to r (reveal (hide (U.raise_val (reveal x))))
-      as ghost_pcm_pts_to r (U.raise_val (reveal x));
-  fold (pts_to #a #p r x);
-  r
-}
-```
+let alloc #a #p x = ghost_alloc #_ #(PR.raise p) (U.raise_val x)
   
 ```pulse
 ghost
@@ -33,24 +20,24 @@ fn read
     (#a:Type u#0)
     (#p:pcm a)
     (r:gref p)
-    (x:erased a)
+    (x:a)
     (f: (v:a{FStar.PCM.compatible #a p (reveal x) v}
           -> GTot (y:a{compatible p y v /\
                         FStar.PCM.frame_compatible p x v y})))
 requires pts_to r x
-returns v: (v:erased a { compatible p x v /\ p.refine v })
+returns v:(v:a { compatible p x v /\ p.refine v })
 ensures pts_to r (f v) 
 {
   unfold pts_to;
-  rewrite ghost_pcm_pts_to #_ #(PR.raise p) r (U.raise_val u#0 u#1 (reveal x))
-      as ghost_pcm_pts_to #_ #(PR.raise p) r (reveal (hide (U.raise_val (reveal x))));
-  let v = ghost_read #_ #(PR.raise u#0 u#1 p) r (U.raise_val (reveal x)) (PR.raise_refine u#0 u#1 p x f);
+  rewrite ghost_pcm_pts_to #_ #(PR.raise p) r (U.raise_val u#0 u#1 x)
+      as ghost_pcm_pts_to #_ #(PR.raise p) r (reveal (hide (U.raise_val x)));
+  let v = ghost_read #_ #(PR.raise u#0 u#1 p) r (U.raise_val x) (PR.raise_refine u#0 u#1 p x f);
   let v = U.downgrade_val (Ghost.reveal v);
   with _v. 
    rewrite ghost_pcm_pts_to #(U.raise_t u#0 u#1 a) #(PR.raise p) r _v
-        as ghost_pcm_pts_to #_ #(PR.raise p) r (U.raise_val u#0 u#1 (f (reveal (hide v))));
-  fold (pts_to r (f (reveal (hide v))));
-  hide v
+        as ghost_pcm_pts_to #_ #(PR.raise p) r (U.raise_val u#0 u#1 (f v));
+  fold (pts_to r (f v));
+  v
 }
 ```
 
@@ -65,42 +52,41 @@ let read_simple
     (#a:Type)
     (#p:pcm a)
     (r:gref p)
-    (#x:erased a)
+    (#x:a)
 = read #a #p r x (identity_frame_compatible p x)
 
 let write
     (#a:Type)
     (#p:pcm a)
     (r:gref p)
-    (x y:Ghost.erased a)
+    (x y:a)
     (f:FStar.PCM.frame_preserving_upd p x y)
 : stt_ghost unit
     emp_inames
     (pts_to r x)
     (fun _ -> pts_to r y)
-= ghost_write #_ #(PR.raise p) r (U.raise_val (reveal x)) (U.raise_val (reveal y))
+= ghost_write #_ #(PR.raise p) r (U.raise_val x) (U.raise_val y)
                  (PR.raise_upd f)
 
 let share
     (#a:Type)
     (#pcm:pcm a)
     (r:gref pcm)
-    (v0:FStar.Ghost.erased a)
-    (v1:FStar.Ghost.erased a{composable pcm v0 v1})
+    (v0:a)
+    (v1:a{composable pcm v0 v1})
 : stt_ghost unit
     emp_inames
     (pts_to r (v0 `op pcm` v1))
     (fun _ -> pts_to r v0 ** pts_to r v1)
-= ghost_share #_ #(PR.raise pcm) r (U.raise_val (reveal v0)) (U.raise_val (reveal v1))
+= ghost_share #_ #(PR.raise pcm) r (U.raise_val v0) (U.raise_val v1)
 
 let gather
     (#a:Type)
     (#pcm:pcm a)
     (r:gref pcm)
-    (v0:FStar.Ghost.erased a)
-    (v1:FStar.Ghost.erased a)
+    (v0 v1:a)
 : stt_ghost (squash (composable pcm v0 v1))
     emp_inames
     (pts_to r v0 ** pts_to r v1)
     (fun _ -> pts_to r (op pcm v0 v1))
-= ghost_gather #_ #(PR.raise pcm) r (U.raise_val (reveal v0)) (U.raise_val (reveal v1))
+= ghost_gather #_ #(PR.raise pcm) r (U.raise_val v0) (U.raise_val v1)
